systems/ChordPromises.v
@@ -1,4 +1,5 @@
 Require Import List.
+Import ListNotations.
 
 Require Import InfSeqExt.infseq.
 
@@ -9,6 +10,7 @@ Require Import Chord.ChordProof.
 Require Import Chord.ChordSemantics.
 Import ChordSemantics.
 Import ConstrainedChord.
+Require Import Chord.ChordValidPointersInvariant.
 
 Definition nodes_have_live_succs (gst : global_state) : Prop :=
   forall h st,
@@ -23,5 +25,46 @@ Theorem nodes_always_have_live_succs :
     lb_execution ex ->
     reachable_st ex.(hd).(occ_gst) ->
     always (now (fun occ => nodes_have_live_succs occ.(occ_gst))) ex.
+Proof.
+Admitted.
+
+Definition circular_wait : occurrence -> Prop.
+Admitted.
+
+Definition successor_nodes_valid (gst : global_state) : Prop :=
+  forall h p st,
+    In p (succ_list st) ->
+    sigma gst h = Some st ->
+    In (addr_of p) (nodes gst) /\
+    exists pst, sigma gst (addr_of p) = Some pst /\
+           joined pst = true.
+
+Lemma successor_nodes_always_valid :
+  forall gst,
+    reachable_st gst ->
+    successor_nodes_valid gst.
+Proof.
+Admitted.
+
+
+Lemma wf_ptr_succ_list_invariant :
+  forall gst h st p rest,
+    reachable_st gst ->
+    sigma gst h = Some st ->
+    succ_list st = p :: rest ->
+    wf_ptr p.
+Proof.
+Admitted.
+
+Definition nonempty_succ_lists (gst : global_state) : Prop :=
+  forall h st,
+    sigma gst h = Some st ->
+    joined st = true ->
+    succ_list st <> [].
+
+Lemma nodes_have_nonempty_succ_lists :
+  forall gst,
+    reachable_st gst ->
+    nonempty_succ_lists gst.
 Proof.
 Admitted.
